Refactor ADT and Hlist, clean up code
Make ADT and Hlist (mostly, pending Common) independent of Why3
Refactor into separate Util files
Delete some uneeded lemmas

proofs/ADT/ADT.v
@@ -1,148 +1,12 @@
-Require Import Coq.Strings.String.
-Require Import Coq.Lists.List.
-Require Import Coq.Bool.Bool.
-Require Import Coq.Logic.Eqdep.
-Require Import Coq.Logic.Eqdep_dec.
-(*Require Import Coq.Logic.EqdepFacts.*)
-Import ListNotations.
+Require Export Coq.Strings.String.
 
-From mathcomp Require all_ssreflect. (*fintype finfun.*)
+(*Require Import Coq.Logic.EqdepFacts.*)
+(*Import ListNotations.*)
+Require Export Hlist.
+Require Export ADTUtil.
+Require Export Coq.Logic.FunctionalExtensionality.
 
 Set Bullet Behavior "Strict Subproofs".
-
-Coercion proj_sumbool (A B: Prop) (H: {A} + {B}) : bool :=
-  if H then true else false.
-Coercion is_true : bool >-> Sortclass.
-
-(*TODO: Separate file*)
-Section Util.
-
-Inductive ForallT {A: Type} (P: A -> Type) : list A -> Type :=
-  | ForallT_nil: ForallT P nil
-  | ForallT_cons: forall {x: A} {l: list A},
-    P x -> ForallT P l -> ForallT P (x :: l).
-
-Lemma ForallT_hd {A: Type} {P: A -> Type} {x: A} {l: list A}:
-  ForallT P (x :: l) ->
-  P x.
-Proof.
-  intros. inversion X; subst. apply X0.
-Qed.
-
-Lemma ForallT_tl {A: Type} {P: A -> Type} {x: A} {l: list A}:
-  ForallT P (x :: l) ->
-  ForallT P l.
-Proof.
-  intros. inversion X; auto.
-Qed.
-
-(*This awkward definition satisfies Coq's positivity checker
-  for nested induction, unlike the normal one*)
-  Definition map2 {A B C: Type} :=
-    fun (f: A -> B -> C) =>
-      fix map2 (l1: list A) : list B -> list C :=
-        match l1 with
-        | nil => fun l2 => nil
-        | x1 :: t1 =>
-          fun l2 =>
-          match l2 with
-          | nil => nil
-          | x2 :: t2 => f x1 x2 :: map2 t1 t2
-          end
-        end.
-
-Lemma bool_irrelevance (b: bool) (p1 p2: b): p1 = p2.
-Proof.
-  apply UIP_dec, bool_dec.
-Qed.
-
-Lemma is_false {P: Type}: false -> P.
-Proof.
-discriminate.
-Qed.
-
-Definition proj2_bool {b1 b2: bool} (x: b1 && b2) : b2 :=
-  proj2 (andb_prop _ _ x).
-
-Definition proj1_bool {b1 b2: bool} (x: b1 && b2) : b1 :=
-  proj1 (andb_prop _ _ x).
-
-Lemma NoDup_map_in: forall {A B: Type} {f: A -> B} {l: list A} {x1 x2: A},
-  NoDup (map f l) ->
-  In x1 l -> In x2 l ->
-  f x1 = f x2 ->
-  x1 = x2.
-Proof.
-  intros A B f l x1 x2 Hn Hin1 Hin2 Hfeq.
-  induction l; simpl.
-  - destruct Hin1.
-  - simpl in *. destruct Hin1; destruct Hin2; subst; auto;
-    inversion Hn; subst;
-    try solve[exfalso; apply H2; 
-      (rewrite Hfeq + rewrite <- Hfeq); rewrite in_map_iff; 
-      (solve[exists x2; auto] + solve[exists x1; auto])].
-    apply IHl; assumption.
-Qed.
-
-End Util.
-
-(*TODO: move*)
-(*In many places, we need the type {x : T | in x l} and the type T is
-  decidable. We give utilities here for this type*)
-Module InType.
-
-(*First do without ssreflect, do we need?*)
-Section InTypeDef.
-Variable (T: Set). (*Set?*)
-Variable (T_dec: forall (x y: T), {x = y} + {x <> y}).
-
-Definition inb (x: T) (l: list T) : bool :=
-  fold_right (fun y acc => ((T_dec x y) || acc)) false l.
-
-Lemma inb_spec (x: T) (l: list T): reflect (In x l) (inb x l).
-Proof.
-  induction l; simpl.
-  - apply ReflectF; auto.
-  - apply ssr.ssrbool.orPP; auto.
-    destruct (T_dec x a); subst; simpl;
-    [apply ReflectT | apply ReflectF]; auto.
-Qed.
-
-Definition in_type (l: list T) : Set :=
-  { x : T | inb x l }.
-
-Definition build_in_type {x: T} {l: list T} (x_in: inb x l): in_type l :=
-  exist _ x x_in.
-
-Definition in_type_extra (l: list T) (f: T -> Set) : Set :=
-  {t: in_type l & f (proj1_sig t)}.
-
-Definition build_extra {l: list T} (x: in_type l) {f: T -> Set} (y: f (proj1_sig x)) :
-  in_type_extra l f :=
-  existT _ x y.
-
-Lemma in_type_eq (l: list T) (x y: in_type l):
-  x = y <-> proj1_sig x = proj1_sig y.
-Proof.
-  destruct x as [x inx]; destruct y as [y iny]; simpl.
-  split; intros.
-  - apply EqdepFacts.eq_sig_fst in H; assumption.
-  - subst. assert (inx = iny) by (apply bool_irrelevance); subst; reflexivity.
-Qed.
-
-Lemma in_type_dec (l: list T) (x y: in_type l): {x = y} + {x <> y}.
-Proof.
-  destruct (T_dec (proj1_sig x) (proj1_sig y)).
-  - left. apply in_type_eq in e; auto.
-  - right. intro C; subst; contradiction.
-Qed.
-
-(*TODO: prove finite and stuff? If so, need ssreflect*)
-End InTypeDef.
-
-End InType.
-
-Import InType.
 
 Section ADT.
 
@@ -151,8 +15,6 @@ Section ADT.
 Variable base: Set.
 Variable base_inhab: base.
 Variable base_dec: forall (x y: base), {x = y} + {x <> y}.
-
-(*TODO: use ssreflect? and eqType*)
 
 (*Type variables are represented by nats, representing their position in
   the list of arguments: ex, for (either A B), we have Left, which takes
@@ -229,38 +91,19 @@ Record adt : Set := {a_name: string; a_params: nat; a_constrs: list constr}.
 (*Mutual blocks consist of a list of ADTs*)
 Record mut : Set := {m_adts: list adt}.
 
-(*TODO: is there ssreflect to do this?
-  "apply" at bottom: ex: if we have P1 -> P1 -> Q and lemma P -> Q,
-    transforms to P1 -> P2 -> P*)
-
 (*Decidable Equality*)
 Section Eq.
 Import all_ssreflect. 
 
-(*TODO: move both of these to some "Util"*)
-
-(*A version of "reflect_dec" with better computational behavior:
-  it reduces even if the "reflect" predicate is opaque*)
-Definition reflect_dec' {P} {b} (H: reflect P b): {P} + {~P} :=
-  match b as b1 return b = b1 -> _ with
-  | true => fun Heq => left (elimT H Heq)
-  | false => fun Hneq => right (elimF H Hneq)
-  end erefl.
-
 Definition typesym_eqb (t1 t2: typesym) : bool :=
   String.eqb (ts_name t1) (ts_name t2) &&
   Nat.eqb (ts_args t1) (ts_args t2).
-
-Ltac reflF :=
-  let C := fresh in
-  intros; apply ReflectF; intro C; inversion C; subst; contradiction.
   
 Lemma typesym_eqb_spec (t1 t2: typesym) : reflect (t1 = t2) (typesym_eqb t1 t2).
 Proof.
   rewrite /typesym_eqb.
   case: (String.eqb_spec _ _); last by reflF.
   case: (PeanoNat.Nat.eqb_spec _ _); last by reflF. 
-  (*TODO: ssreflect should be able to do this I am sure*)
   move=> args_eq names_eq; apply ReflectT; move: args_eq names_eq.
   by case: t1; case: t2 => n1 a1 n2 a2/=->->.
 Qed.
@@ -318,28 +161,6 @@ Qed.
 Definition ty_eq_dec (t1 t2: ty): {t1 = t2} + {t1 <> t2} :=
   reflect_dec' (ty_eqb_spec t1 t2).
 
-(*Equality on lists*)
-Fixpoint list_eqb {A: Type} (eq_dec: forall (x y: A), {x = y} + {x <> y})
-(l1 l2: list A) : bool :=
-  match l1, l2 with
-  | x1 :: t1, x2 :: t2 => eq_dec x1 x2 && list_eqb eq_dec t1 t2
-  | nil, nil => true
-  | _, _ => false
-  end.
-
-Lemma list_eqb_spec {A: Type} (eq_dec: forall (x y: A), {x = y} + {x <> y})
-(l1 l2: list A) : reflect (l1 = l2) (list_eqb eq_dec l1 l2).
-Proof.
-  move: l2. elim: l1 => [[/=|/=]|x1 t1 IH [/=|x2 t2/=]]; try by reflF.
-  - by apply ReflectT.
-  - case: (eq_dec x1 x2)=>//=[->|]; last by reflF.
-    by case: (IH t2)=>[->|]; [apply ReflectT | reflF].
-Qed.
-
-Definition list_eq_dec {A: Type} (eq_dec: forall (x y: A), {x = y} + {x <> y})
-(l1 l2: list A) : {l1 = l2} + {l1 <> l2} := reflect_dec' (list_eqb_spec eq_dec l1 l2).
-
-(*The others are much easier*)
 Definition constr_eqb (c1 c2: constr) : bool :=
   String.eqb (c_name c1) (c_name c2) &&
   list_eqb ty_eq_dec (c_args c1) (c_args c2).
@@ -387,7 +208,6 @@ Definition mut_eq_dec (m1 m2: mut): {m1 = m2} + {m1 <> m2} :=
 
 End Eq.
 
-
 (*Basic definitions for W-types*)
 
 Section W.
@@ -409,15 +229,11 @@ Inductive W : I -> Set :=
 
 End W.
 
-(*TODO: move*)
-Inductive empty := .
-
 Section Encode.
 
 (*All encodings for previously-declared (or abstract) type symbols
   are given by a function typs.
   This is allows to return anything when the length of the list is wrong*)
-(*TODO: Type?*)
 Variable (typs: typesym -> list Set -> Set).
 (*The user also specifies how base types (e.g. unit, bool, etc) are
   interpreted*)
@@ -428,15 +244,12 @@ Variable bases_inhab: bases base_inhab.
 (*We encode a particular mutual type:*)
 Variable (m: mut).
 
-(*We now define the type A (build_base):*)
-Section ADef.
+(*Before defining the encoding, we first need an operation to
+  get the ADT from a given type*)
+Section GetADT.
 
-(*TODO: move*)
 (*TODO: when we add functions, this will become more complicated*)
 (*NOTE: this does NOT handle nested types (ex: tree = node of list tree)*)
-
-(*This is a bit of overkill for now (we only want to know if a type symbol
-  is an ADT/mut occurrence), but it will be useful later*)
 Definition typesym_get_adt_aux (ts: typesym) : option adt :=
   fold_right (fun a acc => if string_dec (ts_name ts) (a_name a) then Some a 
     else acc) None (m_adts m).
@@ -476,7 +289,7 @@ Proof.
   destruct (typesym_get_adt_aux ts) eqn : Hty.
   - left. apply (exist _ a). apply typesym_get_adt_aux_some, Hty.
   - right. apply typesym_get_adt_aux_none, Hty.
-Qed. (*TODO: see if need to be Defined*)
+Qed.
 
 Definition is_ind_occ (ind: string) (t: ty) : bool :=
   match t with
@@ -488,17 +301,25 @@ Definition is_ind_occ (ind: string) (t: ty) : bool :=
   | _ => false
   end.
 
-(*Is the type an occurence of any ADT in the mutual block?*)
-(*
-Definition is_mut_occ (t: ty) : bool :=
+Definition is_rec_ty (t: ty) : bool :=
   match t with
-  | ty_app ts tys =>
-    match (typesym_get_adt ts) with
-    | inleft _ => true
-    | inright _ => false
-    end
+  | ty_app ts tys => if typesym_get_adt ts then true else false
   | _ => false
-  end.*)
+  end.
+
+Lemma ind_occ_is_rec_ty {a} {t: ty}:
+  is_ind_occ a t ->
+  is_rec_ty t.
+Proof.
+  unfold is_ind_occ, is_rec_ty.
+  destruct t; auto.
+  destruct (typesym_get_adt t); auto.
+Qed.
+
+End GetADT.
+
+(*We now define the type A (build_base):*)
+Section ADef.
 
 (*A (non-recursive) type is interpreted according to these functions.
   Type variables are defined by a function to be given later*)
@@ -512,15 +333,6 @@ Fixpoint ty_to_set (vars: list Set) (t: ty) : Set :=
     | inright _ => typs ts (map (ty_to_set vars) tys)
     end
   end.
-
-(*Iterated tuple*)
-Fixpoint big_sprod (l: list Set) : Set :=
-  match l with
-  | nil => unit
-  | x :: xs => (x * (big_sprod xs))%type
-  end.
-
-  (*maybe change [ty_to_set] to include the unit part*)
 
 (*The type for a single constructor is an iterated product of the
   representations (ty_to_set) of each of the argument types.
@@ -563,7 +375,7 @@ Definition num_rec_type (a: adt) (tys: list ty)  : Set :=
   {i: nat | Nat.ltb i (length tys) && 
     is_ind_occ (a_name a) (nth i tys ty_d)}.
 
-(*TODO: generalize to bool pred like ssr?*)
+(*Could generalize to bool pred like ssr?*)
 Lemma num_rec_type_eq {a: adt} {tys: list ty}
   (x1 x2: num_rec_type a tys):
   proj1_sig x1 = proj1_sig x2 ->
@@ -607,7 +419,7 @@ Definition get_constr_type (P: list Set) (a: adt) (cs: list constr) (c: constr)
 
 (*Note the weird type of [recs]. This says that we have n instances of 
   [mk_adts P t], where n is the number of times t occurs recursively in
-  c's constructor list. ([pe] just lifts n to the type level)
+  c's constructor list. ([num_rec_type] just lifts n to the type level)
   But we don't just give a list, or an n-tuple/vector, because we need
   to keep track of which index in c's arg list each instance comes from.
   This will be extremely helpful later*)
@@ -619,15 +431,14 @@ Definition make_constr (P: list Set) (a: mut_in_type) (c: constr)
   mkW mut_in_type P _ _
   a (get_constr_type P (proj1_sig a) _ c c_in data) recs.
 
-(*Now that the core encoding is finished, we prove some theorems
-  (maybe helpful to prove induction here instead of later)*)
+(*Now that the core encoding is finished, we prove some theorems*)
 
 Section Theorems.
 
 (*Inversion: For any instance of [mk_adts], we can find the constructor
   and the arguments used to create it*)
 
-(*MUCH easier than before AND no axioms needed*)
+(*No axioms needed*)
 Definition find_constr: forall (a: mut_in_type) (P: list Set) (x: mk_adts P a),
   {c: constr & {t: inb _ constr_eq_dec c (a_constrs (proj1_sig a)) *
     build_constr_base P c * 
@@ -664,8 +475,6 @@ Qed.
 
 (*Injectivity: Constructor_rep is injective*)
 
-
-
 (*Relies on [eq_rect_eq] for case when A does not have decidable equality*)
 Lemma mkW_inj (I: Set) (eqI: forall (x y: I), {x = y} + {x <> y}) 
 (P: list Set) (A: list Set -> I -> Set)
@@ -686,7 +495,7 @@ subst. exists eq_refl. intros. simpl.
 apply inj_pair2 in H1; subst; reflexivity.
 Qed.
 
-(*Relies on UIP for case when A does not have decidable equality*)
+(*Relies on UIP*)
 Lemma constrs_inj: forall (a: mut_in_type) (P: list Set) 
 (c: constr) 
 (c_in: inb _ constr_eq_dec c (a_constrs (proj1_sig a)))
@@ -764,11 +573,10 @@ End Theorems.
   the constructor). Instead we want the constructor encoding to be
   a constructor applied to arguments. To ensure well-typed argumets, 
   we use a heterogenous list*)
-Require Import Hlist. (*TODO factor out Hlist*)
 
 (*The full mapping from types to Sets, where ADT instances are interpreted
   as the corresponding [mk_adts]*)
-(*NOTE: (remove) unlike before, domain of ADT is definitionally equal to
+(*NOTE: unlike previous version, domain of ADT is definitionally equal to
   mk_adts, not propositionally equal. This reduces need for casts*)
 Definition domain (p: list Set) (t: ty) : Set :=
   match t with
@@ -782,41 +590,28 @@ Definition domain (p: list Set) (t: ty) : Set :=
   | _ => ty_to_set p t
   end. 
 
-(*Convert between a [big_sprod] and an [hlist]*)
-
-Fixpoint big_sprod_to_hlist {A: Set} {f: A -> Set} {l: list A} (x: big_sprod (map f l))
-  {struct l} : hlist f l :=
-  match l as l' return big_sprod (map f l') -> hlist f l' with
-  | nil => fun _ => HL_nil _
-  | x :: xs => fun p => HL_cons _ x xs (fst p) (big_sprod_to_hlist (snd p))
-  end x.
-
-Fixpoint hlist_to_big_sprod {A: Set} {f: A -> Set} {l: list A} (h: hlist f l) :
-  big_sprod (map f l) :=
-  match l as l' return hlist f l' -> big_sprod (map f l') with
-  | nil => fun _ => tt
-  | x :: xs => fun h => (hlist_hd h, hlist_to_big_sprod (hlist_tl h))
-  end h.
-
-Lemma hlist_to_big_sprod_inv {A: Set} {f: A -> Set} {l: list A} (x: big_sprod (map f l)):
-  hlist_to_big_sprod (big_sprod_to_hlist x) = x.
+(*This coincides with [ty_to_set] for all non-recursive types*)
+Lemma is_rec_ty_eq {t: ty} (Hrec: is_rec_ty t = false) p:
+  domain p t = ty_to_set p t.
 Proof.
-  induction l; simpl; [| rewrite IHl]; destruct x; reflexivity.
+  destruct t; simpl in *; auto.
+  destruct (typesym_get_adt t); simpl in *; auto.
+  discriminate.
 Qed.
 
-Lemma big_sprod_to_hlist_inv {A: Set} {f: A -> Set} {l: list A} (h: hlist f l):
-  big_sprod_to_hlist (hlist_to_big_sprod h) = h.
+Lemma is_rec_ty_unit {t: ty} (Hrec: is_rec_ty t) p:
+  unit = ty_to_set p t.
 Proof.
-  induction l; simpl.
-  - symmetry. apply hlist_nil.
-  - rewrite IHl. symmetry. apply hlist_inv.
+  destruct t; simpl in *; try discriminate.
+  destruct (typesym_get_adt t); simpl in *; auto.
+  discriminate.
 Qed.
 
 (*Now convert an [hlist] on [domains] to one on [ty_to_set] (ie: remove
   recursive information)*)
 Fixpoint hlist_dom_to_set {p: list Set} {l: list ty} (h: hlist (domain p) l):
   hlist (ty_to_set p) l.
-
+Proof.
   refine (match l as l' return hlist (domain p) l' -> hlist (ty_to_set p) l' with
   | nil => fun _ => HL_nil _
   | x :: xs => fun h => 
@@ -833,25 +628,11 @@ case (typesym_get_adt ts).
 - intros _ y. exact y.
 Defined.
 
-Definition is_rec_ty (t: ty) : bool :=
-  match t with
-  | ty_app ts tys => if typesym_get_adt ts then true else false
-  | _ => false
-  end.
+(*Two theorems about this: behavior on non-recursive and
+  recursive elements*)
 
-Lemma is_rec_ty_eq {t: ty} (Hrec: is_rec_ty t = false) p:
-  domain p t = ty_to_set p t.
-Proof.
-  destruct t; simpl in *; auto.
-  destruct (typesym_get_adt t); simpl in *; auto.
-  discriminate.
-Qed.
-
-Ltac uip_subst e := assert (e = eq_refl) by (apply UIP); subst.
-
-(*Now we prove that, if the ith element of l is non-recursive,
-  [hlist_dom_to_set] is the same as the original list*)
-(*Needs UIP*)
+(*If the ith element of l is non-recursive,
+  [hlist_dom_to_set] is the same as the original list (UIP)*)
 Lemma hlist_dom_to_set_ith_nonrec {p: list Set} {l: list ty} 
   (h: hlist (domain p) l) (i: nat) (d1: ty) (d2: ty_to_set p d1)
   (d3: domain p d1) (Hrec: is_rec_ty (nth i l d1) = false):
@@ -875,14 +656,6 @@ Proof.
         -- intros. uip_subst e. reflexivity.
     + apply IHl; auto.
       apply Arith_prebase.lt_S_n_stt in H; auto.
-Qed.
-
-Lemma is_rec_ty_unit {t: ty} (Hrec: is_rec_ty t) p:
-  unit = ty_to_set p t.
-Proof.
-  destruct t; simpl in *; try discriminate.
-  destruct (typesym_get_adt t); simpl in *; auto.
-  discriminate.
 Qed.
 
 (*And likewise, if the ith element is recursive, [hlist_dom_to_set]
@@ -917,37 +690,6 @@ Definition args_to_constr_base_aux p (l: list ty)
   (a: hlist (domain p) l): build_constr_base_aux p l :=
   hlist_to_big_sprod (hlist_dom_to_set a).
 
-
-(*First, from an hlist of the arguments, build the [build_constr_base].
-  Conceptually this is very simple: just go through and build the tuple with
-  each non-recursive type found*)
-(*It turns out to be better to mostly write this manually; we do not run into
-  dependent pattern matching issues when destructing [typesym_get_adt]*)
-(*Fixpoint args_to_constr_base_aux p (l: list ty)
-  (a: hlist (domain p) l):
-  build_constr_base_aux p l.
-refine(
-  match l as l' return hlist (domain p) l' -> build_constr_base_aux p l' with
-  | nil => fun _ => tt
-  | thd :: ttl => fun a => 
-    let l' := thd :: ttl in 
-    match a in (hlist _ l1) with
-    | HL_nil => tt
-    | HL_cons x tl ahd atl =>
-      match x as x' return (domain p x') -> build_constr_base_aux p (x' :: tl) with
-      | ty_base b => fun ahd => (ahd, args_to_constr_base_aux p tl atl)
-      | ty_var n => fun ahd => (ahd, args_to_constr_base_aux p tl atl)
-      | ty_app ts tys => _
-      end ahd
-    end
-  end a).
-  unfold build_constr_base_aux.
-  simpl in *.
-  case (typesym_get_adt ts).
-  - intros _ _. exact (tt, args_to_constr_base_aux p tl atl).
-  - intros _ y. exact (y, args_to_constr_base_aux p tl atl).
-Defined.*)
-
 Definition args_to_constr_base (p: list Set) (c: constr)
   (a: hlist (domain p) (c_args c)): build_constr_base p c :=
   args_to_constr_base_aux p (c_args c) a.
@@ -959,7 +701,6 @@ Definition dom_d: forall p, domain p ty_d := fun p =>
 Definition ty_set_d: forall p, ty_to_set p ty_d := fun p =>
   bases_inhab.
 
-(*TODO: move*)
 (*We require that all ADT names are unique*)
 (*TODO: change to decidable version*)
 Variable adt_names_uniq: NoDup (map a_name (m_adts m)).
@@ -1016,7 +757,6 @@ case (typesym_get_adt ts).
   set (pack_eq := (proj2 (in_type_eq _ adt_eq_dec (m_adts m) t' t)) a_eq :
   (build_in_type adt adt_eq_dec (proj1 (proj2_sig s))) = t).
   exact (scast (f_equal (mk_adts p) pack_eq) rep).
-  (*exact (eq_rect _ (mk_adts p) rep _ pack_eq).*)
 - intros _ f. exact (is_false f).
 Defined.
 
@@ -1040,60 +780,7 @@ Definition constr_rep (p: list Set) (a: mut_in_type) (c: constr)
   the extra information we included in the types*)
 Section Inverse.
 
-(*TODO: move*)
-Fixpoint gen_hlist_i {A: Type} (f: A -> Type) (l: list A) (d: A)
-  (g: forall (i: nat), Nat.ltb i (length l) -> f (nth i l d)) : hlist f l :=
-  match l as l' return (forall (i: nat), Nat.ltb i (length l') -> f (nth i l' d)) -> hlist f l' with
-  | nil => fun _ => HL_nil _
-  | x :: xs => fun g => HL_cons _ x xs (g 0 eq_refl) (gen_hlist_i f xs d 
-    (fun i Hi => g (S i) Hi))
-  end g.
-
-Lemma gen_hlist_i_nth {A: Type} {f: A -> Type} {l: list A} {d: A}
-  {g: forall (i: nat), Nat.ltb i (length l) -> f (nth i l d)} {i: nat} d2 
-  (Hi: Nat.ltb i (length l)):
-  hnth i (gen_hlist_i f l d g) d d2 = g i Hi.
-Proof.
-  revert g.
-  generalize dependent i. induction l; simpl; intros.
-  - pose proof (ssrbool.elimT (PeanoNat.Nat.ltb_spec0 i 0) Hi).
-    inversion H.
-  - destruct i; auto.
-    + (*Booleans help us to get proof irrelevance here*)
-      f_equal. apply bool_irrelevance.
-    + erewrite IHl. reflexivity.
-Qed. 
-
-(*It is easier to convert to an hlist and use hnth than to find the ith
-  element of a big_tuple directly*)
-
-(*Fixpoint big_sprod_to_hlist (l: list Set) (x: big_sprod l) {struct l}: 
-  hlist (fun (x: Set) => (x: Type)) l :=
-  match l as l' return big_sprod l' -> hlist (fun (x: Set) => (x: Type)) l' with
-  | nil => fun _ => HL_nil _
-  | x :: xs => fun p => HL_cons _ x xs (fst p) (big_sprod_to_hlist xs (snd p))
-  end x.*)
-
-
-(*Get the ith element of a [big_sprod]*)
-Definition big_sprod_ith {A: Set} {f: A -> Set} {l: list A} 
-  (x: big_sprod (map f l)) (i: nat) (d1: A) (d2: f d1) : f (nth i l d1) :=
-  hnth i (big_sprod_to_hlist x) d1 d2.
-
-Lemma build_constr_base_aux_nth_eq (p: list Set) (l: list ty) (i: nat)
-  (Hi: Nat.ltb i (length l))
- (d: Set) (t_d: ty):
-  nth i (map (ty_to_set p) l) d =
-  ty_to_set p (nth i l t_d).
-Proof.
-  (*TODO: move*)
-  erewrite Common.map_nth_inbound.
-  reflexivity.
-  apply(ssrbool.elimT (PeanoNat.Nat.ltb_spec0 _ _) Hi).
-Qed.
-
-(*NOTE: this won't work: these have to be Defined (I think)*)
-
+(*One small result we need relating [typesym_get_adt] and [is_ind_occ]*)
 Lemma typesym_get_adt_ind_occ ts tys ty (Heq: ty = ty_app ts tys) a:
   typesym_get_adt ts = inleft a ->
   is_ind_occ (a_name (proj1_sig a)) ty.
@@ -1105,33 +792,12 @@ intros C. injection C; intros Heq; subst.
 destruct (string_dec _ _); auto.
 Qed.
 
-Lemma typesym_get_adt_mut_occ {p} ts tys (*ty (Heq: ty = ty_app ts tys)*)
-  (bse: ty_to_set p (ty_app ts tys)) b:
-  typesym_get_adt ts = inright b ->
-  typs ts (map (ty_to_set p) tys).
-Proof.
-simpl in bse |- *.
-destruct (typesym_get_adt ts); try discriminate.
-intros; exact bse.
-Qed.
-
-
-Lemma andb_conj {b1 b2: bool} (x: b1) (y: b2): b1 && b2.
-Proof.
-rewrite x, y. reflexivity.
-Qed.
-
-
-(*Think we need dependent type*)
+(*Generate the [hlist] from the [build_constr_base] and recs*)
 Definition constr_ind_to_args_aux (p: list Set) (l: list ty)
   (b: build_constr_base_aux p l)
   (recs: forall t : mut_in_type, num_rec_type (proj1_sig t) l -> mk_adts p t):
-  hlist (domain p) l 
-
-  
-  .
+  hlist (domain p) l.
 refine (gen_hlist_i (domain p) l ty_d _).
-(*Not sure if this will work*)
 refine ( fun i Hi =>
 
 (fun (t: ty) (Heq: t = nth i l ty_d) =>
@@ -1152,7 +818,6 @@ simpl in bse |- *.
 revert bse.
 (*Need info about [ind_occ] later*)
 pose proof (typesym_get_adt_ind_occ ts tys _ (eq_sym Heq)). revert H.
-(*pose proof (typesym_get_adt_mut_occ ts tys bse). revert H.*)
 case (typesym_get_adt ts).
 - intros s Hindocc _.
   (*Have all the info for recs (why we needed Heq)*)
@@ -1161,7 +826,6 @@ case (typesym_get_adt ts).
   exact (recs t' n).
 - intros _ _ bse.
   exact bse.
-
 Defined.
 
 Definition constr_ind_to_args (p: list Set) (c: constr)
@@ -1170,19 +834,12 @@ Definition constr_ind_to_args (p: list Set) (c: constr)
   hlist (domain p) (c_args c) :=
   constr_ind_to_args_aux p (c_args c) b recs.
 
-Ltac gen_scast :=
-  match goal with
-  | |- context [scast ?H ?x] => generalize dependent H
-  end.
-
-  (*If we have [scast Heq1 x] and [scast Heq2 x], write the first
-    in terms of the second*)
-Lemma scast_switch {A B C: Set} (x: A) (Heq1: A = B) (Heq2: A = C):
-  scast Heq1 x = scast (eq_trans (eq_sym Heq2) Heq1) (scast Heq2 x).
-Proof.
-  subst. reflexivity.
-Qed.
-
+(*Before proving the inverse results, we need a few
+  lemmas allowing us to simplify [constr_ind_to_args_aux].
+  In particular, we prove simplifications for the case when
+  (nth i l ty_d) is recursive and non-recursive. These lemmas
+  are tricky because we need to generalize (nth i l ty_d) in
+  very particular ways*)
 
 Lemma is_ind_occ_domain p (a: mut_in_type) (t: ty) 
   (Hind: is_ind_occ (a_name (proj1_sig a)) t):
@@ -1377,26 +1034,6 @@ Proof.
   reflexivity.
 Qed.
 
-Lemma big_sprod_ext {A: Set} {f: A -> Set} (l: list A) 
-  (x1 x2: big_sprod (map f l)) (d1: A) (d2: f d1)
-  (Hext: forall i, i < length l -> big_sprod_ith x1 i d1 d2 = big_sprod_ith x2 i d1 d2):
-  x1 = x2.
-Proof.
-  (*Use inverse functions*)
-  rewrite <- (hlist_to_big_sprod_inv x1), <- (hlist_to_big_sprod_inv x2).
-  f_equal.
-  apply hlist_ext_eq with (d:=d1)(d':=d2).
-  apply Hext.
-Qed.
-
-Lemma ty_to_set_rec p {t: ty}:
-  is_rec_ty t ->
-  ty_to_set p t = unit.
-Proof.
-  destruct t; simpl; try discriminate.
-  destruct (typesym_get_adt); auto; discriminate.
-Qed.
-
 (*Now, the proofs of the inverse:*)
 Lemma constr_ind_args_inv_aux1 {p: list Set} {l: list ty}
 (b: build_constr_base_aux p l)
@@ -1413,7 +1050,7 @@ Proof.
     rewrite (hlist_dom_to_set_ith_rec _ i _ _ Hrec Hi).
     generalize dependent (is_rec_ty_unit Hrec p). 
     generalize dependent (hnth i (big_sprod_to_hlist b) ty_d (ty_set_d p)).
-    rewrite (ty_to_set_rec p Hrec).
+    rewrite <- (is_rec_ty_unit Hrec).
     intros. uip_subst e. destruct t. reflexivity.
   - (*If non-recursive, use previous result*)
     rewrite (hlist_dom_to_set_ith_nonrec _ i _ _ (dom_d p) Hrec Hi).
@@ -1453,6 +1090,8 @@ Proof.
     + intros. exact (is_false i).
 Qed.
 
+(*For the other direction, we need to get information out of the
+  [is_rec_ty] hypothesis to construct the needed [num_rec_type]*)
 Lemma is_rec_ty_get_info {i l} (Hi: i < length l) (Hrec: is_rec_ty (nth i l ty_d)):
   {t: mut_in_type & {x: num_rec_type (proj1_sig t) l | proj1_sig x = i}}.
 Proof.
@@ -1542,8 +1181,6 @@ End Inverse.
 (*And now the 4 conditions, fully:*)
 Section Theorems.
 
-Require Import Coq.Logic.FunctionalExtensionality.
-
 (*Needs funext and UIP*)
 Theorem find_constr_rep {p: list Set} {t: mut_in_type} (x: mk_adts p t):
   {c: constr & {Hf: inb _ constr_eq_dec c (a_constrs (proj1_sig t)) *
@@ -1574,8 +1211,8 @@ Proof.
   apply constrs_disjoint.
 Qed.
 
-(*One more structural lemma (TODO: move) allowing us to replace recs
-  without requiring funext*)
+(*One more lemma about [constr_ind_to_args_aux] 
+  allowing us to replace recs without requiring funext*)
 Lemma constr_ind_to_args_recs_ext {p: list Set} {l: list ty}
   {b} {recs1 recs2}
   (Hext: forall t x, recs1 t x = recs2 t x):
@@ -1589,10 +1226,8 @@ Proof.
   unfold constr_ind_to_args_aux.
   rewrite !gen_hlist_i_nth with (Hi:=Hi').
   simpl.
-  (*generalize dependent (@eq_refl _ (nth i l ty_d)).*)
   generalize dependent (big_sprod_ith b i ty_d (dom_d p)).
   intros t.
-  (*Generalize again*)
   (*Again, we need a more generic lemma*)
   match goal with
   | |- (match nth i l ty_d as t1 in ty return (t1 = nth i l ty_d -> ty_to_set p t1 -> domain p t1)
@@ -1652,15 +1287,6 @@ Proof.
   assumption.
 Qed.
 
-Lemma ind_occ_is_rec_ty {a} {t: ty}:
-  is_ind_occ a t ->
-  is_rec_ty t.
-Proof.
-  unfold is_ind_occ, is_rec_ty.
-  destruct t; auto.
-  destruct (typesym_get_adt t); auto.
-Qed.
-
 Lemma is_ind_occ_twice {a1 a2: mut_in_type} (t: ty):
   is_ind_occ (a_name (proj1_sig a1)) t ->
   is_ind_occ (a_name (proj1_sig a2)) t ->
@@ -1679,7 +1305,7 @@ Proof.
     congruence.
 Qed.
 
-(*Induction*)
+(*Induction - requires funext and UIP*)
 Theorem adt_rep_ind (P: forall (t: mut_in_type) (p: list Set), mk_adts p t -> Prop):
   (forall (t: mut_in_type) (p: list Set) (x: mk_adts p t)
     (c: constr) (c_in:  inb _ constr_eq_dec c (a_constrs (proj1_sig t)))
