proofs/ADT/ADTUtil.v
@@ -1,0 +1,195 @@
+Require Export Coq.Lists.List.
+Require Export Coq.Bool.Bool.
+Require Export Coq.Logic.Eqdep.
+Require Export Coq.Logic.Eqdep_dec.
+Require Export Lia.
+From mathcomp Require all_ssreflect.
+Export ListNotations.
+
+Set Bullet Behavior "Strict Subproofs".
+
+(*Working with Boolean Predicates*)
+
+Coercion proj_sumbool (A B: Prop) (H: {A} + {B}) : bool :=
+  if H then true else false.
+Coercion is_true : bool >-> Sortclass.
+
+Lemma bool_irrelevance (b: bool) (p1 p2: b): p1 = p2.
+Proof.
+  apply UIP_dec, bool_dec.
+Qed.
+
+Lemma is_false {P: Type}: false -> P.
+Proof.
+discriminate.
+Qed.
+
+Lemma andb_conj {b1 b2: bool} (x: b1) (y: b2): b1 && b2.
+Proof.
+rewrite x, y. reflexivity.
+Qed.
+
+Definition proj2_bool {b1 b2: bool} (x: b1 && b2) : b2 :=
+  proj2 (andb_prop _ _ x).
+
+Definition proj1_bool {b1 b2: bool} (x: b1 && b2) : b1 :=
+  proj1 (andb_prop _ _ x).
+
+(*Forall for Type*)
+
+Inductive ForallT {A: Type} (P: A -> Type) : list A -> Type :=
+  | ForallT_nil: ForallT P nil
+  | ForallT_cons: forall {x: A} {l: list A},
+    P x -> ForallT P l -> ForallT P (x :: l).
+
+Lemma ForallT_hd {A: Type} {P: A -> Type} {x: A} {l: list A}:
+  ForallT P (x :: l) ->
+  P x.
+Proof.
+  intros. inversion X; subst. apply X0.
+Qed.
+
+Lemma ForallT_tl {A: Type} {P: A -> Type} {x: A} {l: list A}:
+  ForallT P (x :: l) ->
+  ForallT P l.
+Proof.
+  intros. inversion X; auto.
+Qed.
+
+(*Some list definitions and lemmas*)
+
+(*This awkward definition satisfies Coq's positivity checker
+  for nested induction, unlike the normal one*)
+Definition map2 {A B C: Type} :=
+  fun (f: A -> B -> C) =>
+    fix map2 (l1: list A) : list B -> list C :=
+      match l1 with
+      | nil => fun l2 => nil
+      | x1 :: t1 =>
+        fun l2 =>
+        match l2 with
+        | nil => nil
+        | x2 :: t2 => f x1 x2 :: map2 t1 t2
+        end
+      end.
+
+Lemma NoDup_map_in: forall {A B: Type} {f: A -> B} {l: list A} {x1 x2: A},
+  NoDup (map f l) ->
+  In x1 l -> In x2 l ->
+  f x1 = f x2 ->
+  x1 = x2.
+Proof.
+  intros A B f l x1 x2 Hn Hin1 Hin2 Hfeq.
+  induction l; simpl.
+  - destruct Hin1.
+  - simpl in *. destruct Hin1; destruct Hin2; subst; auto;
+    inversion Hn; subst;
+    try solve[exfalso; apply H2; 
+      (rewrite Hfeq + rewrite <- Hfeq); rewrite in_map_iff; 
+      (solve[exists x2; auto] + solve[exists x1; auto])].
+    apply IHl; assumption.
+Qed.
+
+(*More general than [map_nth] from the standard library because
+  we don't require any knowledge of the default values as long
+  as n is within bounds*)
+Lemma map_nth_inbound: forall {A B: Type} (f: A -> B) (l: list A)
+  (d1 : B) (d2 : A) (n: nat),
+  n < length l ->
+  nth n (List.map f l) d1 = f (nth n l d2).
+Proof.
+  intros A B f l d1 d2. induction l as [|h t IH]; simpl; try lia.
+  intros n Hn.
+  destruct n; auto. 
+  apply IH. lia.
+Qed. 
+
+Inductive empty := .
+
+(*In many places, we need the type {x : T | in x l} and the type T is
+decidable. We give utilities here for this type*)
+
+Section InTypeDef.
+Variable (T: Set).
+Variable (T_dec: forall (x y: T), {x = y} + {x <> y}).
+
+Definition inb (x: T) (l: list T) : bool :=
+  fold_right (fun y acc => ((T_dec x y) || acc)) false l.
+
+Lemma inb_spec (x: T) (l: list T): reflect (In x l) (inb x l).
+Proof.
+  induction l; simpl.
+  - apply ReflectF; auto.
+  - apply ssr.ssrbool.orPP; auto.
+    destruct (T_dec x a); subst; simpl;
+    [apply ReflectT | apply ReflectF]; auto.
+Qed.
+
+Definition in_type (l: list T) : Set :=
+  { x : T | inb x l }.
+
+Definition build_in_type {x: T} {l: list T} (x_in: inb x l): in_type l :=
+  exist _ x x_in.
+
+Definition in_type_extra (l: list T) (f: T -> Set) : Set :=
+  {t: in_type l & f (proj1_sig t)}.
+
+Definition build_extra {l: list T} (x: in_type l) {f: T -> Set} (y: f (proj1_sig x)) :
+  in_type_extra l f :=
+  existT _ x y.
+
+Lemma in_type_eq (l: list T) (x y: in_type l):
+  x = y <-> proj1_sig x = proj1_sig y.
+Proof.
+  destruct x as [x inx]; destruct y as [y iny]; simpl.
+  split; intros.
+  - apply EqdepFacts.eq_sig_fst in H; assumption.
+  - subst. assert (inx = iny) by (apply bool_irrelevance); subst; reflexivity.
+Qed.
+
+Lemma in_type_dec (l: list T) (x y: in_type l): {x = y} + {x <> y}.
+Proof.
+  destruct (T_dec (proj1_sig x) (proj1_sig y)).
+  - left. apply in_type_eq in e; auto.
+  - right. intro C; subst; contradiction.
+Qed.
+
+End InTypeDef.
+
+Ltac reflF :=
+  let C := fresh in
+  intros; apply ReflectF; intro C; inversion C; subst; contradiction.
+
+Section Eq.
+Import all_ssreflect. 
+
+(*A version of "reflect_dec" with better computational behavior:
+it reduces even if the "reflect" predicate is opaque*)
+Definition reflect_dec' {P} {b} (H: reflect P b): {P} + {~P} :=
+  match b as b1 return b = b1 -> _ with
+  | true => fun Heq => left (elimT H Heq)
+  | false => fun Hneq => right (elimF H Hneq)
+  end erefl.
+
+(*Equality on lists*)
+Fixpoint list_eqb {A: Type} (eq_dec: forall (x y: A), {x = y} + {x <> y})
+(l1 l2: list A) : bool :=
+  match l1, l2 with
+  | x1 :: t1, x2 :: t2 => eq_dec x1 x2 && list_eqb eq_dec t1 t2
+  | nil, nil => true
+  | _, _ => false
+  end.
+
+Lemma list_eqb_spec {A: Type} (eq_dec: forall (x y: A), {x = y} + {x <> y})
+(l1 l2: list A) : reflect (l1 = l2) (list_eqb eq_dec l1 l2).
+Proof.
+  move: l2. elim: l1 => [[/=|/=]|x1 t1 IH [/=|x2 t2/=]]; try by reflF.
+  - by apply ReflectT.
+  - case: (eq_dec x1 x2)=>//=[->|]; last by reflF.
+    by case: (IH t2)=>[->|]; [apply ReflectT | reflF].
+Qed.
+
+Definition list_eq_dec {A: Type} (eq_dec: forall (x y: A), {x = y} + {x <> y})
+(l1 l2: list A) : {l1 = l2} + {l1 <> l2} := reflect_dec' (list_eqb_spec eq_dec l1 l2).
+
+End Eq.
